1.<br/>

(a) T⇒(D∧Y)<br/>

(b) D⇒¬Y<br/>

(c) ¬D⇒¬T<br/>

(d) T⇒¬(D∧Y)<br/>

(e) T⇒¬D∧Y<br/>

(f) T⇒Y∧¬D<br/>

(g) (T⇒Y∧D) ∨(T⇒¬Y∧¬D) (may be wrong)<br/> **Teacher's answer: T ⇒ (D⇔Y)**<br/>

(h) (T⇒Y∧¬D)∨(T⇒¬Y∧D) (right)<br/>

 **Teacher's answer: T ⇒ [(D∨Y)∧(D∧Y)]**<br/>

2.<br/>

F, T, T<br/>

F, F, F<br/>

T, T, T<br/>

T, T, T<br/>

3.<br/>

from the aspect of result,  " φ ⇒ ψ" is equal to "¬φ ∨ ψ"<br/>

but why?<br/>

 **Teacher's answer:  " φ ⇒ ψ" is equivalent to "¬φ ∨ ψ"**<br/>

4.<br/>

F, T, F, F<br/>

T, F, T, T<br/>

F, T, F, F<br/>

T, T, F, F<br/>

5.<br/>

from the aspect of result,  "¬(φ ⇒ ψ)" is equal to " φ ∧ ¬ψ"<br/>

but why?<br/>

 **Teacher's answer:  " ¬(φ ⇒ ψ)" is equivalent to "φ ∧ ¬ψ"**<br/>